all the examples

Examples/STLC/Term.lean
@@ -7,7 +7,7 @@ namespace STLC
 
 inductive Ty where
 | base : Ty
-| arrow : Ty -> Ty
+| arrow : Ty -> Ty -> Ty
 
 notation "★" => Ty.base
 infixr:64 " -:> " => Ty.arrow
@@ -20,145 +20,134 @@ inductive Term where
 prefix:max "#" => Term.var
 notation "λ[" A "]" t => Term.lam A t
 
-#leansubst var Term.var
-#leansubst bind Term at pos 1 in Term.lam
+@[coe]
+def Term.from_action : Action Term -> Term
+| re y => var y
+| su t => t
 
-set_option diagnostics true
+@[simp]
+theorem Term.from_action_id {n} : from_action (𝐬0.act n) = var n := by
+  simp [from_action]
 
-#leansubst generate Term
+@[simp]
+theorem Term.from_action_succ {n} : from_action (𝐬1.act n) = var (n + 1) := by
+  simp [from_action]
 
--- @[simp]
--- instance : HSMul Term Term Term where
---   hSMul := Term.app
+@[simp]
+theorem Term.from_acton_re {n} : from_action (re n) = var n := by simp [from_action]
 
--- @[coe]
--- def Term.from_action : Action Term -> Term
--- | re y => var y
--- | su t => t
+@[simp]
+theorem Term.from_action_su {t} : from_action (su t) = t := by simp [from_action]
 
--- @[simp]
--- theorem Term.from_action_id {n} : from_action (𝐬0.act n) = var n := by
---   simp [from_action]
+instance : Coe (Action Term) Term where
+  coe := Term.from_action
 
--- @[simp]
--- theorem Term.from_action_succ {n} : from_action (𝐬1.act n) = var (n + 1) := by
---   simp [from_action]
+@[simp]
+def Term.rmap (r : RenVec [Term]) : Term -> Term
+| var x => var (r.1.act x)
+| app t1 t2 => app (t1.rmap r) (t2.rmap r)
+| λ[A] t => λ[A] t.rmap $ r.lift [1]
 
--- @[simp]
--- theorem Term.from_acton_re {n} : from_action (re n) = var n := by simp [from_action]
+instance : RenMap Term [Term] where
+  rmap := Term.rmap
 
--- @[simp]
--- theorem Term.from_action_su {t} : from_action (su t) = t := by simp [from_action]
+instance : RenSuffix Term [] := ⟨⟩
+instance : RenMap Term [] where
+  rmap _ := id
 
--- instance : Coe (Action Term) Term where
---   coe := Term.from_action
+@[simp]
+theorem Term.rmap_empty {t : Term} {r : RenVec []} : t⟨r,⟩ = t := by
+  simp only [RenMap.rmap, id]
 
--- @[simp]
--- def Term.rmap (r : RenVec [Term]) : Term -> Term
--- | var x => var (r.1.act x)
--- | app t1 t2 => app (t1.rmap r) (t2.rmap r)
--- | λ[A] t => λ[A] t.rmap $ r.lift [1]
+@[reducible, simp]
+instance instRenMapAll_Term : RenMapAll [Term] := .cons .nil
 
--- instance : RenMap Term [Term] where
---   rmap := Term.rmap
+@[simp]
+theorem Term.rmap_fix {r : RenVec [Term]} {t : Term} : rmap r t = t⟨r,⟩ := by simp [RenMap.rmap]
 
--- instance : RenSuffix Term [] := ⟨⟩
--- instance : RenMap Term [] where
---   rmap _ := id
+@[simp]
+theorem Term.rmap_var {x} {r : RenVec [Term]} : (#x)⟨r,⟩ = .var (r.1.act x) := by
+  simp only [RenMap.rmap]; rw [rmap]
 
--- @[simp]
--- theorem Term.rmap_empty {t : Term} {r : RenVec []} : t⟨r,⟩ = t := by
---   simp only [RenMap.rmap, id]
+@[simp]
+theorem Term.rmap_app {t1 t2 : Term} {r : RenVec [Term]} : (app t1 t2)⟨r,⟩ = app t1⟨r,⟩ t2⟨r,⟩ := by
+  simp only [RenMap.rmap]; rw [rmap]
 
--- @[reducible, simp]
--- instance instRenMapAll_Term : RenMapAll [Term] := .cons .nil
+@[simp]
+theorem Term.rmap_lam {A t} {r : RenVec [Term]} : (λ[A] t)⟨r,⟩ = λ[A] t⟨r.lift [1],⟩ := by
+  simp only [RenMap.rmap]; rw [rmap]
 
--- @[simp]
--- theorem Term.rmap_fix {r : RenVec [Term]} {t : Term} : rmap r t = t⟨r,⟩ := by simp [RenMap.rmap]
+@[simp]
+theorem Term.from_action_rmap {t : Action Term} {r : RenVec [Term]}
+  : (from_action t)⟨r,⟩ = from_action t⟨r,⟩
+:= by cases t <;> simp
 
--- @[simp]
--- theorem Term.rmap_var {x} {r : RenVec [Term]} : (#x)⟨r,⟩ = .var (r.1.act x) := by
---   simp only [RenMap.rmap]; rw [rmap]
+instance : RenMapEmpty Term where
+  apply_empty := by intro s; simp
 
--- @[simp]
--- theorem Term.rmap_app {t1 t2 : Term} {r : RenVec [Term]} : (app t1 t2)⟨r,⟩ = app t1⟨r,⟩ t2⟨r,⟩ := by
---   simp only [RenMap.rmap]; rw [rmap]
+instance : RenMapId Term [Term] where
+  apply_id := by subst_solve_id
 
--- @[simp]
--- theorem Term.rmap_lam {A t} {r : RenVec [Term]} : (λ[A] t)⟨r,⟩ = λ[A] t⟨r.lift [1],⟩ := by
---   simp only [RenMap.rmap]; rw [rmap]
+instance : RenMapCompose Term [Term] where
+  apply_compose := by subst_solve_compose
 
--- @[simp]
--- theorem Term.from_action_rmap {t : Action Term} {r : RenVec [Term]}
---   : (from_action t)⟨r,⟩ = from_action t⟨r,⟩
--- := by cases t <;> simp
+@[simp]
+def Term.smap (σ : SubstVec [Term]) : Term -> Term
+| var x => σ.1.act x
+| app t1 t2 => app (t1.smap σ) (t2.smap σ)
+| λ[A] t => λ[A] t.smap $ σ.lift [1]
 
--- instance : RenMapEmpty Term where
---   apply_empty := by intro s; simp
+instance : SubstMap Term [Term] where
+  smap := Term.smap
 
--- instance : RenMapId Term [Term] where
---   apply_id := by subst_solve_id
+instance : SubstSuffix Term [] := ⟨⟩
+instance : SubstMap Term [] where
+  smap _ := id
 
--- instance : RenMapCompose Term [Term] where
---   apply_compose := by subst_solve_compose
+@[simp]
+theorem Term.smap_empty {t : Term} {σ : SubstVec []} : t[σ,] = t := by
+  simp only [SubstMap.smap, id]
 
--- @[simp]
--- def Term.smap (σ : SubstVec [Term]) : Term -> Term
--- | var x => σ.1.act x
--- | app t1 t2 => app (t1.smap σ) (t2.smap σ)
--- | λ[A] t => λ[A] t.smap $ σ.lift [1]
+@[reducible, simp]
+instance instSubstMapAll_Ty : SubstMapAll [Term] := .cons .nil
 
--- instance : SubstMap Term [Term] where
---   smap := Term.smap
+@[simp]
+theorem Term.smap_fix {σ : SubstVec [Term]} {t : Term} : smap σ t = t[σ,] := by simp [SubstMap.smap]
 
--- instance : SubstSuffix Term [] := ⟨⟩
--- instance : SubstMap Term [] where
---   smap _ := id
+@[simp]
+theorem Term.smap_var {x} {σ : SubstVec [Term]} : (#x)[σ,] = from_action (σ.1.act x) := by
+  simp only [SubstMap.smap]; rw [smap]
 
--- @[simp]
--- theorem Term.smap_empty {t : Term} {σ : SubstVec []} : t[σ,] = t := by
---   simp only [SubstMap.smap, id]
+@[simp]
+theorem Term.smap_app {t1 t2 : Term} {σ : SubstVec [Term]} : (app t1 t2)[σ,] = app t1[σ,] t2[σ,] := by
+  simp only [SubstMap.smap]; rw [smap]
 
--- @[reducible, simp]
--- instance instSubstMapAll_Ty : SubstMapAll [Term] := .cons .nil
+@[simp]
+theorem Term.smap_lam {A t} {σ : SubstVec [Term]} : (λ[A] t)[σ,] = λ[A] t[σ.lift [1],] := by
+  simp only [SubstMap.smap]; rw [smap]
 
--- @[simp]
--- theorem Term.smap_fix {σ : SubstVec [Term]} {t : Term} : smap σ t = t[σ,] := by simp [SubstMap.smap]
+@[simp]
+theorem Term.from_action_smap {t : Action Term} {σ : SubstVec [Term]}
+  : (from_action t)[σ,] = from_action t[σ,]
+:= by cases t <;> simp
 
--- @[simp]
--- theorem Term.smap_var {x} {σ : SubstVec [Term]} : (#x)[σ,] = from_action (σ.1.act x) := by
---   simp only [SubstMap.smap]; rw [smap]
+instance : SubstMapEmpty Term where
+  apply_empty := by intro s; simp
 
--- @[simp]
--- theorem Term.smap_app {t1 t2 : Term} {σ : SubstVec [Term]} : (app t1 t2)[σ,] = app t1[σ,] t2[σ,] := by
---   simp only [SubstMap.smap]; rw [smap]
+instance : SubstMapId Term [Term] where
+  apply_id := by subst_solve_id
 
--- @[simp]
--- theorem Term.smap_lam {A t} {σ : SubstVec [Term]} : (λ[A] t)[σ,] = λ[A] t[σ.lift [1],] := by
---   simp only [SubstMap.smap]; rw [smap]
+instance : SubstMapStable Term [Term] where
+  apply_stable := by subst_solve_stable
 
--- @[simp]
--- theorem Term.from_action_smap {t : Action Term} {σ : SubstVec [Term]}
---   : (from_action t)[σ,] = from_action t[σ,]
--- := by cases t <;> simp
+instance : SubstMapRenComposeLeft Term [Term] where
+  apply_ren_compose_left := by subst_solve_compose
 
--- instance : SubstMapEmpty Term where
---   apply_empty := by intro s; simp
+instance : SubstMapRenComposeRight Term [Term] where
+  apply_ren_compose_right := by subst_solve_compose
 
--- instance : SubstMapId Term [Term] where
---   apply_id := by subst_solve_id
-
--- instance : SubstMapStable Term [Term] where
---   apply_stable := by subst_solve_stable
-
--- instance : SubstMapRenComposeLeft Term [Term] where
---   apply_ren_compose_left := by subst_solve_compose
-
--- instance : SubstMapRenComposeRight Term [Term] where
---   apply_ren_compose_right := by subst_solve_compose
-
--- instance : SubstMapCompose Term [Term] where
---   apply_compose := by subst_solve_compose
+instance : SubstMapCompose Term [Term] where
+  apply_compose := by subst_solve_compose
 
 
 end STLC
