Examples/SystemFWithNat/Term.lean
@@ -12,6 +12,9 @@ inductive Ty where
 | all : Ty -> Ty
 | nat : Ty
 
+#leansubst var Ty.var
+#leansubst bind Ty at pos 0 in Ty.all
+
 inductive Term where
 | var : Nat -> Term
 | app : Term -> Term -> Term
@@ -22,8 +25,6 @@ inductive Term where
 | succ : Term -> Term
 | nrec (motive : Ty) (z : Term) (s : Term) (n : Term) : Term -- binds 2 Term's in s
 
-#leansubst var Ty.var
-#leansubst bind Ty at pos 0 in Ty.all
 
 #leansubst var Term.var
 #leansubst bind Term at pos 1 in Term.lam
@@ -32,768 +33,768 @@ inductive Term where
 
 --set_option diagnostics true
 
-#leansubst generate Ty, Term
-
--- Checking Ty --
-#print Ty.from_action
-#print Ty.from_action_id
-#print Ty.from_action_succ
-#print Ty.from_action_re
-#print Ty.from_action_su
-
-#check (inferInstance : Coe (Action Ty) Ty)
-
-#print Ty.rmap
-#print Ty.rmap._f
-
-#check (inferInstance : RenMap Ty [Ty])
-
-#print Ty.rmap_fix
-#print Ty.rmap_empty -- should be removed
-
-#check (inferInstance : RenSuffix Ty [])
-#check (inferInstance : RenMap Ty [])
-#check (inferInstance : RenMapAll [Ty])
-
-#print Ty.rmap_var
-#print Ty.rmap_arrow
-#print Ty.rmap_all
-#print Ty.rmap_nat
-#print Ty.from_action_rmap
-
-#check (inferInstance : RenMapEmpty Ty)
-#check (inferInstance : RenMapId Ty [Ty])
-#check (inferInstance : RenMapCompose Ty [Ty])
-
-#print Ty.smap
-#print Ty.smap._f
-
-#check (inferInstance : SubstMap Ty [Ty])
-
-#print Ty.smap_fix
-#print Ty.smap_empty -- to be removed
-
-#check (inferInstance : SubstSuffix Ty [])
-#check (inferInstance : SubstMap Ty [])
-#check (inferInstance : SubstMapAll [Ty])
-
-#print Ty.smap_var
-#print Ty.smap_arrow
-#print Ty.smap_all
-#print Ty.smap_nat
-#print Ty.from_action_smap
-
-#check (inferInstance : SubstMapEmpty Ty)
-#check (inferInstance : SubstMapId Ty [Ty])
-#check (inferInstance : SubstMapStable Ty [Ty])
-#check (inferInstance : SubstMapRenComposeLeft Ty [Ty])
-#check (inferInstance : SubstMapRenComposeRight Ty [Ty])
-#check (inferInstance : SubstMapCompose Ty [Ty])
-
--- Checking Term --
-#print Term.from_action
-#print Term.from_action_id
-#print Term.from_action_succ
-#print Term.from_action_re
-#print Term.from_action_su
-
-#check (inferInstance : Coe (Action Term) Term)
-
--- rmap
-#print Term.rmap
-#print Term.rmap._f
-
-#check (inferInstance : RenMap Term [Term, Ty])
-#check (inferInstance : RenSuffix Term [Ty])
-#check (inferInstance : RenMap Term [Ty])
-#check (inferInstance : RenMap Term [Term])
-#check (inferInstance : RenSuffix Term [])
-#check (inferInstance : RenMap Term [])
-#check (inferInstance : RenMapAll [Term])
-#check (inferInstance : RenMapAll [Term, Ty])
-
-#print Term.rmap_empty -- to be removed
-#print Term.rmap_fix
-
-#print Term.rmap_term_var
-#print Term.rmap_term_app
-#print Term.rmap_term_lam
-#print Term.rmap_term_tapp
-#print Term.rmap_term_tlam
-#print Term.rmap_term_zero
-#print Term.rmap_term_succ
-#print Term.rmap_term_nrec
-
-#print Term.rmap_ty_var
-#print Term.rmap_ty_app
-#print Term.rmap_ty_lam
-#print Term.rmap_ty_tapp
-#print Term.rmap_ty_tlam
-#print Term.rmap_ty_zero
-#print Term.rmap_ty_succ
-#print Term.rmap_ty_nrec
-
-#print Term.rmap_term_ty_var
-#print Term.rmap_term_ty_app
-#print Term.rmap_term_ty_lam
-#print Term.rmap_term_ty_tapp
-#print Term.rmap_term_ty_tlam
-#print Term.rmap_term_ty_zero
-#print Term.rmap_term_ty_succ
-#print Term.rmap_term_ty_nrec
-
-#print Term.from_action_rmap
-#print Term.from_action_rmap0
-#print Term.from_action_rmap1
-
-#check (inferInstance : RenMapEmpty Term)
-#check (inferInstance : RenMapVecDef Term Term [Ty])
-#check (inferInstance : RenMapId Term [Term, Ty])
-#check (inferInstance : RenMapCompose Term [Term, Ty])
-#check (inferInstance : RenMapVecDef Term Term [])
-#check (inferInstance : RenMapId Term [Term])
-#check (inferInstance : RenMapCompose Term [Term])
-#check (inferInstance : RenMapId Term [Ty])
-#check (inferInstance : RenMapCompose Term [Ty])
-
--- smap
-#print Term.smap
-#print Term.smap._f
-
-#check (inferInstance : SubstMap Term [Term, Ty])
-#check (inferInstance : SubstSuffix Term [Ty])
-#check (inferInstance : SubstMap Term [Ty])
-#check (inferInstance : SubstMap Term [Term])
-#check (inferInstance : SubstSuffix Term [])
-#check (inferInstance : SubstMap Term [])
-#check (inferInstance : SubstMapAll [Term])
-#check (inferInstance : SubstMapAll [Term, Ty])
-
-#print Term.smap_empty -- remove
-#print Term.smap_fix
-
-#print Term.smap_term_var
-#print Term.smap_term_app
-#print Term.smap_term_lam
-#print Term.smap_term_tapp
-#print Term.smap_term_tlam
-#print Term.smap_term_zero
-#print Term.smap_term_succ
-#print Term.smap_term_nrec
-
-#print Term.smap_ty_var
-#print Term.smap_ty_app
-#print Term.smap_ty_lam
-#print Term.smap_ty_tapp
-#print Term.smap_ty_tlam
-#print Term.smap_ty_zero
-#print Term.smap_ty_succ
-#print Term.smap_ty_nrec
-
-#print Term.smap_term_ty_var
-#print Term.smap_term_ty_app
-#print Term.smap_term_ty_lam
-#print Term.smap_term_ty_tapp
-#print Term.smap_term_ty_tlam
-#print Term.smap_term_ty_zero
-#print Term.smap_term_ty_succ
-#print Term.smap_term_ty_nrec
-
-#print Term.from_action_smap
-#print Term.from_action_smap0
-#print Term.from_action_smap1
-
-#check (inferInstance : SuffixCommuteRenRen Term [Ty])
-#check (inferInstance : SuffixCommuteRenSub Term [Ty])
-#check (inferInstance : SuffixCommuteSubRen Term [Ty])
-#check (inferInstance : SubstMapEmpty Term)
-
-#check (inferInstance : SubstMapVecDef Term Term [Ty])
-#check (inferInstance : SubstMapId Term [Term, Ty])
-#check (inferInstance : SubstMapStable Term [Term, Ty])
-#check (inferInstance : SubstMapRenComposeLeft Term [Term, Ty])
-#check (inferInstance : SubstMapRenComposeRight Term [Term, Ty])
-
-#check (inferInstance : SubstMapVecDef Term Term [])
-#check (inferInstance : SubstMapId Term [Term])
-#check (inferInstance : SubstMapStable Term [Term])
-#check (inferInstance : SubstMapRenComposeLeft Term [Term])
-#check (inferInstance : SubstMapRenComposeRight Term [Term])
-
-#check (inferInstance : SubstMapId Term [Ty])
-#check (inferInstance : SubstMapStable Term [Ty])
-#check (inferInstance : SubstMapRenComposeLeft Term [Ty])
-#check (inferInstance : SubstMapRenComposeRight Term [Ty])
-
-#check (inferInstance : SubstMapCompose Term [Term, Ty])
-#check (inferInstance : SubstMapCompose Term [Ty])
-#check (inferInstance : SubstMapCompose Term [Term])
-
--- ----------------------------------------------------------------------------------------------------
--- -- Ty Renaming & Substitution
--- ----------------------------------------------------------------------------------------------------
--- @[coe]
--- def Ty.from_action : Action Ty -> Ty
--- | re y => var y
--- | su t => t
-
--- @[simp]
--- theorem Ty.from_action_id {n} : from_action (𝐬0.act n) = var n := by
---   simp [from_action]
-
--- @[simp]
--- theorem Ty.from_action_succ {n} : from_action (𝐬1.act n) = var (n + 1) := by
---   simp [from_action]
-
--- @[simp]
--- theorem Ty.from_action_re {n} : from_action (re n) = var n := by simp [from_action]
-
--- @[simp]
--- theorem Ty.from_action_su {t} : from_action (su t) = t := by simp [from_action]
-
--- instance : Coe (Action Ty) Ty where
---   coe := Ty.from_action
-
--- @[simp]
--- def Ty.rmap (r : RenVec [Ty]) : Ty -> Ty
--- | var x => var (r.1.act x)
--- | nat => nat
--- | arrow t1 t2 => arrow (t1.rmap r) (t2.rmap r)
--- | all t => all $ t.rmap $ r.lift [1]
-
--- instance : RenMap Ty [Ty] where
---   rmap := Ty.rmap
-
--- @[simp]
--- theorem Ty.rmap_fix {r : RenVec [Ty]} {t : Ty} : rmap r t = t⟨r,⟩ := by simp [RenMap.rmap]
-
--- instance : RenSuffix Ty [] := ⟨⟩
--- instance : RenMap Ty [] where
---   rmap _ := id
-
--- @[reducible, simp]
--- instance instRenMapAll_Ty : RenMapAll [Ty] := .cons .nil
-
--- @[simp]
--- theorem Ty.rmap_var {x} {r : RenVec [Ty]} : (var x)⟨r,⟩ = .var (r.1.act x) := by
---   simp only [RenMap.rmap]; rw [rmap]
-
--- @[simp]
--- theorem Ty.rmap_nat {r : RenVec [Ty]} : (nat)⟨r,⟩ = nat := by
---   simp only [RenMap.rmap]; rw [rmap]
-
--- @[simp]
--- theorem Ty.rmap_arrow {t1 t2 : Ty} {r : RenVec [Ty]} : (arrow t1 t2)⟨r,⟩ = arrow t1⟨r,⟩ t2⟨r,⟩ := by
---   simp only [RenMap.rmap]; rw [rmap]
-
--- @[simp]
--- theorem Ty.rmap_all {t} {r : RenVec [Ty]} : (all t)⟨r,⟩ = all t⟨r.lift [1],⟩ := by
---   simp only [RenMap.rmap]; rw [rmap]
-
--- @[simp]
--- theorem Ty.from_action_rmap {t : Action Ty} {r : RenVec [Ty]}
---   : (from_action t)⟨r,⟩ = from_action t⟨r,⟩
--- := by cases t <;> simp
-
--- instance : RenMapEmpty Ty where
---   apply_empty := by intro s; simp [RenMap.rmap]
-
--- instance : RenMapId Ty [Ty] where
---   apply_id := by subst_solve_id
-
--- instance : RenMapCompose Ty [Ty] where
---   apply_compose := by subst_solve_compose
-
--- @[simp]
--- def Ty.smap (σ : SubstVec [Ty]) : Ty -> Ty
--- | var x => σ.1.act x
--- | nat => nat
--- | arrow t1 t2 => arrow (t1.smap σ) (t2.smap σ)
--- | all t => all $ t.smap $ σ.lift [1]
-
--- instance : SubstMap Ty [Ty] where
---   smap := Ty.smap
-
--- @[simp]
--- theorem Ty.smap_fix {σ : SubstVec [Ty]} {t : Ty} : smap σ t = t[σ,] := by simp [SubstMap.smap]
-
--- instance : SubstSuffix Ty [] := ⟨⟩
--- instance : SubstMap Ty [] where
---   smap _ := id
-
--- @[reducible, simp]
--- instance instSubstMapAll_Ty : SubstMapAll [Ty] := .cons .nil
-
--- @[simp]
--- theorem Ty.smap_var {x} {σ : SubstVec [Ty]} : (var x)[σ,] = σ.1.act x := by
---   simp only [SubstMap.smap]; rw [smap]
-
--- @[simp]
--- theorem Ty.smap_nat {σ : SubstVec [Ty]} : (nat)[σ,] = nat := by
---   simp only [SubstMap.smap]; rw [smap]
-
--- @[simp]
--- theorem Ty.smap_arrow {t1 t2 : Ty} {σ : SubstVec [Ty]} : (arrow t1 t2)[σ,] = arrow t1[σ,] t2[σ,] := by
---   simp only [SubstMap.smap]; rw [smap]
-
--- @[simp]
--- theorem Ty.smap_all {t} {σ : SubstVec [Ty]} : (all t)[σ,] = all t[σ.lift [1],] := by
---   simp only [SubstMap.smap]; rw [smap]
-
--- @[simp]
--- theorem Ty.from_action_smap {t : Action Ty} {σ : SubstVec [Ty]}
---   : (from_action t)[σ,] = from_action t[σ,]
--- := by cases t <;> simp
-
--- instance : SubstMapEmpty Ty where
---   apply_empty := by intro s; simp [SubstMap.smap]
-
--- instance : SubstMapId Ty [Ty] where
---   apply_id := by subst_solve_id
-
--- instance : SubstMapStable Ty [Ty] where
---   apply_stable := by subst_solve_stable
-
--- instance : SubstMapRenComposeLeft Ty [Ty] where
---   apply_ren_compose_left := by subst_solve_compose
-
--- instance : SubstMapRenComposeRight Ty [Ty] where
---   apply_ren_compose_right := by subst_solve_compose
-
--- instance : SubstMapCompose Ty [Ty] where
---   apply_compose := by subst_solve_compose
-
--- ----------------------------------------------------------------------------------------------------
--- -- Term Renaming & Substitution
--- ----------------------------------------------------------------------------------------------------
-
--- @[coe]
--- def Term.from_action : Action Term -> Term
--- | re y => var y
--- | su t => t
-
--- @[simp, grind =]
--- theorem Term.from_action_id {n} : from_action (𝐬0.act n) = var n := by
---   simp [from_action]
-
--- @[simp, grind =]
--- theorem Term.from_action_succ {n} : from_action (𝐬1.act n) = var (n + 1) := by
---   simp [from_action]
-
--- @[simp, grind =]
--- theorem Term.from_acton_re {n} : from_action (re n) = var n := by simp [from_action]
-
--- @[simp, grind =]
--- theorem Term.from_action_su {t} : from_action (su t) = t := by simp [from_action]
-
--- instance : Coe (Action Term) Term where
---   coe := Term.from_action
-
--- @[simp]
--- def Term.rmap (r : RenVec [Term, Ty]) : Term -> Term
--- | var x => var (r.1.act x)
--- | app t1 t2 => app (t1.rmap r) (t2.rmap r)
--- | lam A t => lam A⟨r.2.1⟩ (t.rmap $ r.lift [1, 0])
--- | tapp t A => tapp (t.rmap r) A⟨r.2.1⟩
--- | tlam t => tlam (t.rmap $ r.lift [0, 1])
--- | zero => zero
--- | succ t => succ (t.rmap r)
--- | nrec motive z s n => nrec motive⟨r.2.1⟩ (z.rmap r) (s.rmap $ r.lift [2, 1]) (n.rmap r)
-
--- instance : RenMap Term [Term, Ty] where
---   rmap := Term.rmap
-
--- @[simp]
--- theorem Term.rmap_fix {r : RenVec [Term, Ty]} {t : Term} : rmap r t = t⟨r,⟩ := by simp [RenMap.rmap]
-
--- @[simp]
--- theorem Term.rmap_term_ty_var {x} {r : RenVec [Term, Ty]} : (var x)⟨r,⟩ = var (r.1.act x) := rfl
-
--- @[simp]
--- theorem Term.rmap_term_ty_app {t1 t2} {r : RenVec [Term, Ty]} : (app t1 t2)⟨r,⟩ = app t1⟨r,⟩ t2⟨r,⟩ := by
---   simp only [RenMap.rmap]; rw [rmap]
-
--- @[simp]
--- theorem Term.rmap_term_ty_lam'' {A t} {r : RenVec [Term, Ty]}
---   : (lam A t)⟨r,⟩ = lam A⟨r.2.1⟩ t⟨r.lift [1, 0],⟩
--- := by simp only [RenMap.rmap]; rw [rmap]; try simp
-
--- @[simp]
--- theorem Term.rmap_term_ty_tapp {t1 t2} {r : RenVec [Term, Ty]}
---   : (tapp t1 t2)⟨r,⟩ = tapp t1⟨r,⟩ t2⟨r.2.1⟩
--- := by simp only [RenMap.rmap]; rw [rmap]; try simp
-
--- @[simp]
--- theorem Term.rmap_term_ty_tlam {t} {r : RenVec [Term, Ty]} : (tlam t)⟨r,⟩ = tlam t⟨r.lift [0, 1],⟩ := by
---   simp only [RenMap.rmap]; rw [rmap]; try simp
-
--- @[simp]
--- theorem Term.rmap_term_ty_zero {r : RenVec [Term, Ty]} : zero⟨r,⟩ = zero := by
---   simp only [RenMap.rmap]; rw [rmap]; try simp
-
--- @[simp]
--- theorem Term.rmap_term_ty_succ {t} {r : RenVec [Term, Ty]} : (succ t)⟨r,⟩ = succ t⟨r,⟩ := by
---   simp only [RenMap.rmap]; rw [rmap]; try simp
-
--- @[simp]
--- theorem Term.rmap_term_ty_nrec {m z s n} {r : RenVec [Term, Ty]}
---   : (nrec m z s n)⟨r,⟩ = nrec m⟨r.2.1⟩ z⟨r,⟩ s⟨r.lift [2, 1],⟩ n⟨r,⟩
--- := by simp only [RenMap.rmap]; rw [rmap]; try simp
-
--- instance : RenSuffix Term [Ty] := ⟨⟩
--- instance : RenMap Term [Ty] where
---   rmap r := Term.rmap (Ren.id Term, r.1, .nil)
-
--- @[simp]
--- theorem Term.rmap_ty_var {x} {r : RenVec [Ty]} : (var x)⟨r,⟩ = var x := by
---   simp only [RenMap.rmap]; rw [rmap]; try simp
-
--- @[simp]
--- theorem Term.rmap_ty_app {t1 t2} {r : RenVec [Ty]} : (app t1 t2)⟨r,⟩ = app t1⟨r,⟩ t2⟨r,⟩ := by
---   simp only [RenMap.rmap]; rw [rmap]; try simp
-
--- @[simp]
--- theorem Term.rmap_ty_lam {A t} {r : RenVec [Ty]}
---   : (lam A t)⟨r,⟩ = lam A⟨r.1⟩ t⟨r,⟩
--- := by simp only [RenMap.rmap]; rw [rmap]; try simp
-
--- @[simp]
--- theorem Term.rmap_ty_tapp {t1 t2} {r : RenVec [Ty]}
---   : (tapp t1 t2)⟨r,⟩ = tapp t1⟨r,⟩ t2⟨r.1⟩
--- := by simp only [RenMap.rmap]; rw [rmap]; try simp
-
--- @[simp]
--- theorem Term.rmap_ty_tlam {t} {r : RenVec [Ty]} : (tlam t)⟨r,⟩ = tlam t⟨r.lift [1],⟩ := by
---   simp only [RenMap.rmap]; rw [rmap]; try simp
-
--- @[simp]
--- theorem Term.rmap_ty_zero {r : RenVec [Ty]} : zero⟨r,⟩ = zero := by
---   simp only [RenMap.rmap]; rw [rmap]; try simp
-
--- @[simp]
--- theorem Term.rmap_ty_succ {t} {r : RenVec [Ty]} : (succ t)⟨r,⟩ = succ t⟨r,⟩ := by
---   simp only [RenMap.rmap]; rw [rmap]; try simp
-
--- @[simp]
--- theorem Term.rmap_ty_nrec {m z s n} {r : RenVec [Ty]}
---   : (nrec m z s n)⟨r,⟩ = nrec m⟨r.1⟩ z⟨r,⟩ s⟨r.lift [1],⟩ n⟨r,⟩
--- := by simp only [RenMap.rmap]; rw [rmap]; try simp
-
--- instance : RenMap Term [Term] where
---   rmap r := Term.rmap (r.1, Ren.id Ty, .nil)
-
--- @[simp]
--- theorem Term.rmap_term_var {x} {r : RenVec [Term]} : (var x)⟨r,⟩ = var (r.1.act x) := by
---   simp only [RenMap.rmap]; rw [rmap]; try simp
-
--- @[simp]
--- theorem Term.rmap_term_app {t1 t2} {r : RenVec [Term]} : (app t1 t2)⟨r,⟩ = app t1⟨r,⟩ t2⟨r,⟩ := by
---   simp only [RenMap.rmap]; rw [rmap]; try simp
-
--- @[simp]
--- theorem Term.rmap_term_lam' {A t} {r : RenVec [Term]}
---   : (lam A t)⟨r,⟩ = lam A t⟨r.lift [1],⟩
--- := by simp only [RenMap.rmap]; rw [rmap]; try simp
-
--- @[simp]
--- theorem Term.rmap_term_tapp {t1 t2} {r : RenVec [Term]}
---   : (tapp t1 t2)⟨r,⟩ = tapp t1⟨r,⟩ t2
--- := by simp only [RenMap.rmap]; rw [rmap]; try simp
-
--- @[simp]
--- theorem Term.rmap_term_tlam {t} {r : RenVec [Term]} : (tlam t)⟨r,⟩ = tlam t⟨r,⟩ := by
---   simp only [RenMap.rmap]; rw [rmap]; try simp
-
--- @[simp]
--- theorem Term.rmap_term_zero {r : RenVec [Term]} : zero⟨r,⟩ = zero := by
---   simp only [RenMap.rmap]; rw [rmap]; try simp
-
--- @[simp]
--- theorem Term.rmap_term_succ {t} {r : RenVec [Term]} : (succ t)⟨r,⟩ = succ t⟨r,⟩ := by
---   simp only [RenMap.rmap]; rw [rmap]; try simp
-
--- @[simp]
--- theorem Term.rmap_term_nrec {m z s n} {r : RenVec [Term]}
---   : (nrec m z s n)⟨r,⟩ = nrec m z⟨r,⟩ s⟨r.lift [2],⟩ n⟨r,⟩
--- := by simp only [RenMap.rmap]; rw [rmap]; try simp
-
--- @[simp]
--- theorem Term.from_action_rmap {t : Action Term} {r : RenVec [Term, Ty]}
---   : (from_action t)⟨r,⟩ = from_action t⟨r,⟩
--- := by cases t <;> simp [from_action]
-
--- @[simp]
--- theorem Term.from_action_rmap0 {t : Action Term} {r : RenVec [Term]}
---   : (from_action t)⟨r,⟩ = from_action t⟨r,⟩
--- := by cases t <;> simp [from_action]
-
--- @[simp]
--- theorem Term.from_action_rmap1 {t : Action Term} {r : RenVec [Ty]}
---   : (from_action t)⟨r,⟩ = from_action t⟨r,⟩
--- := by cases t <;> simp [from_action]
-
--- instance : RenSuffix Term [] := ⟨⟩
--- instance : RenMap Term [] where
---   rmap _ := id
-
--- @[reducible, simp]
--- instance instRenMapAll_Term : RenMapAll [Term] := .cons .nil
-
--- @[reducible, simp]
--- instance instRenMapAll_Term_Ty : RenMapAll [Term, Ty] := .cons instRenMapAll_Ty
-
--- instance : RenMapEmpty Term where
---   apply_empty := by intro s; simp [RenMap.rmap]
-
--- instance : RenMapVecDef Term Term [Ty] where
---   apply_vecdef := by intro s r; induction s generalizing r <;> simp [*]
-
--- instance : RenMapId Term [Term, Ty] where
---   apply_id := by subst_solve_id
-
--- instance : RenMapCompose Term [Term, Ty] where
---   apply_compose := by subst_solve_compose
-
--- instance : RenMapVecDef Term Term [] where
---   apply_vecdef := by intro s r; induction s generalizing r <;> simp [*]
-
--- instance : RenMapId Term [Term] where
---   apply_id := by subst_solve_id
-
--- instance : RenMapCompose Term [Term] where
---   apply_compose := by subst_solve_compose
-
--- instance : RenMapId Term [Ty] where
---   apply_id := by subst_solve_id
-
--- instance : RenMapCompose Term [Ty] where
---   apply_compose := by subst_solve_compose
-
--- @[simp]
--- def Term.smap (σ : SubstVec [Term, Ty]) : Term -> Term
--- | var x => σ.1.act x
--- | app t1 t2 => app (t1.smap σ) (t2.smap σ)
--- | lam A t => lam A[σ.2.1] (t.smap $ σ.lift [1, 0])
--- | tapp t A => tapp (t.smap σ) A[σ.2.1]
--- | tlam t => tlam (t.smap $ σ |> .lift [0, 1] |> .ren Term [Ty] (𝐫1, .nil) 0 rfl)
--- | zero => zero
--- | succ t => succ (t.smap σ)
--- | nrec motive z s n =>
---   nrec motive[σ.2.1] (z.smap σ) (s.smap $ σ |> .lift [2, 1] |> .ren Term [Ty] (𝐫1, .nil) 0 rfl) (n.smap σ)
-
--- instance : SubstMap Term [Term, Ty] where
---   smap := Term.smap
-
--- @[simp]
--- theorem Term.smap_fix {σ : SubstVec [Term, Ty]} {t : Term} : smap σ t = t[σ,] := by
---   simp [SubstMap.smap]
-
--- @[simp]
--- theorem Term.smap_term_ty_var {x} {σ : SubstVec [Term, Ty]} : (var x)[σ,] = σ.1.act x := by
---   simp only [SubstMap.smap]; rw [smap]; try simp
-
--- @[simp]
--- theorem Term.smap_term_ty_app {t1 t2} {σ : SubstVec [Term, Ty]} : (app t1 t2)[σ,] = app t1[σ,] t2[σ,] := by
---   simp only [SubstMap.smap]; rw [smap]; try simp
-
--- @[simp]
--- theorem Term.smap_term_ty_lam {A t} {σ : SubstVec [Term, Ty]}
---   : (lam A t)[σ,] = lam A[σ.2.1] t[σ.lift [1, 0],]
--- := by simp only [SubstMap.smap]; rw [smap]; try simp
-
--- @[simp]
--- theorem Term.smap_term_ty_tapp {t1 t2} {σ : SubstVec [Term, Ty]}
---   : (tapp t1 t2)[σ,] = tapp t1[σ,] t2[σ.2.1]
--- := by simp only [SubstMap.smap]; rw [smap]; try simp
-
--- @[simp]
--- theorem Term.smap_term_ty_tlam {t} {σ : SubstVec [Term, Ty]}
---   : (tlam t)[σ,] = tlam t[σ |> .lift [0, 1] |> .ren Term [Ty] (𝐫1, .nil) 0 rfl,]
--- := by simp only [SubstMap.smap]; rw [smap]; try simp
-
--- @[simp]
--- theorem Term.smap_term_ty_zero {σ : SubstVec [Term, Ty]} : zero[σ,] = zero := by
---   simp only [SubstMap.smap]; rw [smap]; try simp
-
--- @[simp]
--- theorem Term.smap_term_ty_succ {t} {σ : SubstVec [Term, Ty]} : (succ t)[σ,] = succ t[σ,] := by
---   simp only [SubstMap.smap]; rw [smap]; try simp
-
--- @[simp]
--- theorem Term.smap_term_ty_nrec {m z s n} {σ : SubstVec [Term, Ty]}
---   : (nrec m z s n)[σ,] = nrec m[σ.2.1] z[σ,] s[σ |> .lift [2, 1] |> .ren Term [Ty] (𝐫1, .nil) 0 rfl,] n[σ,]
--- := by simp only [SubstMap.smap]; rw [smap]; try simp
-
--- @[simp]
--- theorem Term.from_action_smap {t : Action Term} {σ : SubstVec [Term, Ty]}
---   : (from_action t)[σ,] = from_action t[σ,]
--- := by cases t <;> simp [from_action]
-
--- instance : SubstSuffix Term [Ty] := ⟨⟩
--- @[simp]
--- instance : SubstMap Term [Ty] where
---   smap σ := Term.smap (Subst.id Term, σ.1, .nil)
-
--- @[simp]
--- theorem Term.smap_ty_var {x} {σ : SubstVec [Ty]} : (var x)[σ,] = var x := by
---   simp only [SubstMap.smap]; rw [smap]; try simp
-
--- @[simp]
--- theorem Term.smap_ty_app {t1 t2} {σ : SubstVec [Ty]} : (app t1 t2)[σ,] = app t1[σ,] t2[σ,] := by
---   simp only [SubstMap.smap]; rw [smap]; try simp
-
--- @[simp]
--- theorem Term.smap_ty_lam {A t} {σ : SubstVec [Ty]}
---   : (lam A t)[σ,] = lam A[σ.1] t[σ,]
--- := by simp only [SubstMap.smap]; rw [smap]; try simp
-
--- @[simp]
--- theorem Term.smap_ty_tapp {t1 t2} {σ : SubstVec [Ty]}
---   : (tapp t1 t2)[σ,] = tapp t1[σ,] t2[σ.1]
--- := by simp only [SubstMap.smap]; rw [smap]; try simp
-
--- @[simp]
--- theorem Term.smap_ty_tlam {t} {σ : SubstVec [Ty]}
---   : (tlam t)[σ,] = tlam t[σ |> .lift [1],]
--- := by simp only [SubstMap.smap]; rw [smap]; try simp
-
--- @[simp]
--- theorem Term.smap_ty_zero {σ : SubstVec [Ty]} : zero[σ,] = zero := by
---   simp only [SubstMap.smap]; rw [smap]; try simp
-
--- @[simp]
--- theorem Term.smap_ty_succ {t} {σ : SubstVec [Ty]} : (succ t)[σ,] = succ t[σ,] := by
---   simp only [SubstMap.smap]; rw [smap]; try simp
-
--- @[simp]
--- theorem Term.smap_ty_nrec {m z s n} {σ : SubstVec [Ty]}
---   : (nrec m z s n)[σ,] = nrec m[σ.1] z[σ,] s[σ |> .lift [1],] n[σ,]
--- := by simp only [SubstMap.smap]; rw [smap]; try simp
-
--- @[simp]
--- theorem Term.from_action_smap1 {t : Action Term} {σ : SubstVec [Ty]}
---   : (from_action t)[σ,] = from_action t[σ,]
--- := by cases t <;> simp [from_action]
-
--- @[simp]
--- instance : SubstMap Term [Term] where
---   smap σ := Term.smap (σ.1, Subst.id Ty, .nil)
-
--- @[simp]
--- theorem Term.smap_term_var {x} {σ : SubstVec [Term]} : (var x)[σ,] = σ.1.act x := by
---   simp only [SubstMap.smap]; rw [smap]; try simp
-
--- @[simp]
--- theorem Term.smap_term_app {t1 t2} {σ : SubstVec [Term]} : (app t1 t2)[σ,] = app t1[σ,] t2[σ,] := by
---   simp only [SubstMap.smap]; rw [smap]; try simp
-
--- @[simp]
--- theorem Term.smap_term_lam {A t} {σ : SubstVec [Term]}
---   : (lam A t)[σ,] = lam A t[σ.lift [1],]
--- := by simp only [SubstMap.smap]; rw [smap]; try simp
-
--- @[simp]
--- theorem Term.smap_term_tapp {t1 t2} {σ : SubstVec [Term]}
---   : (tapp t1 t2)[σ,] = tapp t1[σ,] t2
--- := by simp only [SubstMap.smap]; rw [smap]; try simp
-
--- @[simp]
--- theorem Term.smap_term_tlam {t} {σ : SubstVec [Term]}
---   : (tlam t)[σ,] = tlam t[σ |> .ren Term [Ty] (𝐫1, .nil) 0 rfl,]
--- := by simp only [SubstMap.smap]; rw [smap]; try simp
-
--- @[simp]
--- theorem Term.smap_term_zero {σ : SubstVec [Term]} : zero[σ,] = zero := by
---   simp only [SubstMap.smap]; rw [smap]; try simp
-
--- @[simp]
--- theorem Term.smap_term_succ {t} {σ : SubstVec [Term]} : (succ t)[σ,] = succ t[σ,] := by
---   simp only [SubstMap.smap]; rw [smap]; try simp
-
--- @[simp]
--- theorem Term.smap_term_nrec {m z s n} {σ : SubstVec [Term]}
---   : (nrec m z s n)[σ,] = nrec m z[σ,] s[σ |> .lift [2] |> .ren Term [Ty] (𝐫1, .nil) 0 rfl,] n[σ,]
--- := by simp only [SubstMap.smap]; rw [smap]; try simp
-
--- @[simp]
--- theorem Term.from_action_smap0 {t : Action Term} {σ : SubstVec [Term]}
---   : (from_action t)[σ,] = from_action t[σ,]
--- := by cases t <;> simp [from_action]
-
--- instance : SubstSuffix Term [] := ⟨⟩
--- instance : SubstMap Term [] where
---   smap _ := id
-
--- @[reducible, simp]
--- instance instSubstMapAll_Term : SubstMapAll [Term] := .cons .nil
-
--- @[reducible, simp]
--- instance instSubstMapAll_Term_Ty : SubstMapAll [Term, Ty] := .cons instSubstMapAll_Ty
-
--- instance : SubstMapEmpty Term where
---   apply_empty := by intro s; simp [SubstMap.smap]
-
--- instance : SubstMapVecDef Term Term [] where
---   apply_vecdef := by intro s σ; induction s generalizing σ <;> simp [*]
-
--- -- The `[Ty]` Suffix:
--- instance : SuffixCommuteRenRen Term [Ty] where
---   ren_ren := by subst_solve_compose
-
--- instance : SuffixCommuteRenSub Term [Ty] where
---   ren_sub := by subst_solve_compose
-
--- instance : SuffixCommuteSubRen Term [Ty] where
---   sub_ren := by subst_solve_compose
-
--- instance : SubstMapVecDef Term Term [Ty] where
---   apply_vecdef := by intro s σ; induction s generalizing σ <;> simp [*]
-
--- instance : SubstMapId Term [Ty] where
---   apply_id := by subst_solve_id
-
--- instance : SubstMapStable Term [Ty] where
---   apply_stable := by sorry --subst_solve_stable
-
--- instance : SubstMapRenComposeLeft Term [Ty] where
---   apply_ren_compose_left := by subst_solve_compose
-
--- instance : SubstMapRenComposeRight Term [Ty] where
---   apply_ren_compose_right := by subst_solve_compose
-
--- instance : SubstMapCompose Term [Ty] where
---   apply_compose := by subst_solve_compose
-
--- -- The `[Term]` Singleton:
--- instance : SubstMapId Term [Term] where
---   apply_id := by subst_solve_id
-
--- instance : SubstMapStable Term [Term] where
---   apply_stable := by sorry --subst_solve_stable
-
--- instance : SubstMapRenComposeLeft Term [Term] where
---   apply_ren_compose_left := by subst_solve_compose
-
--- instance : SubstMapRenComposeRight Term [Term] where
---   apply_ren_compose_right := by subst_solve_compose
-
--- instance : SubstMapCompose Term [Term] where
---   apply_compose := by subst_solve_compose
-
--- -- The `[Term, Ty]` Original:
--- instance : SubstMapId Term [Term, Ty] where
---   apply_id := by subst_solve_id
-
--- instance : SubstMapStable Term [Term, Ty] where
---   apply_stable := by sorry --subst_solve_stable
-
--- instance : SubstMapRenComposeLeft Term [Term, Ty] where
---   apply_ren_compose_left := by subst_solve_compose
-
--- instance : SubstMapRenComposeRight Term [Term, Ty] where
---   apply_ren_compose_right := by subst_solve_compose
-
--- instance : SubstMapCompose Term [Term, Ty] where
---   apply_compose := by subst_solve_compose
+-- #leansubst generate Ty, Term
+
+-- -- Checking Ty --
+-- #print Ty.from_action
+-- #print Ty.from_action_id
+-- #print Ty.from_action_succ
+-- #print Ty.from_action_re
+-- #print Ty.from_action_su
+
+-- #check (inferInstance : Coe (Action Ty) Ty)
+
+-- #print Ty.rmap
+-- #print Ty.rmap._f
+
+-- #check (inferInstance : RenMap Ty [Ty])
+
+-- #print Ty.rmap_fix
+-- #print Ty.rmap_empty -- should be removed
+
+-- #check (inferInstance : RenSuffix Ty [])
+-- #check (inferInstance : RenMap Ty [])
+-- #check (inferInstance : RenMapAll [Ty])
+
+-- #print Ty.rmap_var
+-- #print Ty.rmap_arrow
+-- #print Ty.rmap_all
+-- #print Ty.rmap_nat
+-- #print Ty.from_action_rmap
+
+-- #check (inferInstance : RenMapEmpty Ty)
+-- #check (inferInstance : RenMapId Ty [Ty])
+-- #check (inferInstance : RenMapCompose Ty [Ty])
+
+-- #print Ty.smap
+-- #print Ty.smap._f
+
+-- #check (inferInstance : SubstMap Ty [Ty])
+
+-- #print Ty.smap_fix
+-- #print Ty.smap_empty -- to be removed
+
+-- #check (inferInstance : SubstSuffix Ty [])
+-- #check (inferInstance : SubstMap Ty [])
+-- #check (inferInstance : SubstMapAll [Ty])
+
+-- #print Ty.smap_var
+-- #print Ty.smap_arrow
+-- #print Ty.smap_all
+-- #print Ty.smap_nat
+-- #print Ty.from_action_smap
+
+-- #check (inferInstance : SubstMapEmpty Ty)
+-- #check (inferInstance : SubstMapId Ty [Ty])
+-- #check (inferInstance : SubstMapStable Ty [Ty])
+-- #check (inferInstance : SubstMapRenComposeLeft Ty [Ty])
+-- #check (inferInstance : SubstMapRenComposeRight Ty [Ty])
+-- #check (inferInstance : SubstMapCompose Ty [Ty])
+
+-- -- Checking Term --
+-- #print Term.from_action
+-- #print Term.from_action_id
+-- #print Term.from_action_succ
+-- #print Term.from_action_re
+-- #print Term.from_action_su
+
+-- #check (inferInstance : Coe (Action Term) Term)
+
+-- -- rmap
+-- #print Term.rmap
+-- #print Term.rmap._f
+
+-- #check (inferInstance : RenMap Term [Term, Ty])
+-- #check (inferInstance : RenSuffix Term [Ty])
+-- #check (inferInstance : RenMap Term [Ty])
+-- #check (inferInstance : RenMap Term [Term])
+-- #check (inferInstance : RenSuffix Term [])
+-- #check (inferInstance : RenMap Term [])
+-- #check (inferInstance : RenMapAll [Term])
+-- #check (inferInstance : RenMapAll [Term, Ty])
+
+-- #print Term.rmap_empty -- to be removed
+-- #print Term.rmap_fix
+
+-- #print Term.rmap_term_var
+-- #print Term.rmap_term_app
+-- #print Term.rmap_term_lam
+-- #print Term.rmap_term_tapp
+-- #print Term.rmap_term_tlam
+-- #print Term.rmap_term_zero
+-- #print Term.rmap_term_succ
+-- #print Term.rmap_term_nrec
+
+-- #print Term.rmap_ty_var
+-- #print Term.rmap_ty_app
+-- #print Term.rmap_ty_lam
+-- #print Term.rmap_ty_tapp
+-- #print Term.rmap_ty_tlam
+-- #print Term.rmap_ty_zero
+-- #print Term.rmap_ty_succ
+-- #print Term.rmap_ty_nrec
+
+-- #print Term.rmap_term_ty_var
+-- #print Term.rmap_term_ty_app
+-- #print Term.rmap_term_ty_lam
+-- #print Term.rmap_term_ty_tapp
+-- #print Term.rmap_term_ty_tlam
+-- #print Term.rmap_term_ty_zero
+-- #print Term.rmap_term_ty_succ
+-- #print Term.rmap_term_ty_nrec
+
+-- #print Term.from_action_rmap
+-- #print Term.from_action_rmap0
+-- #print Term.from_action_rmap1
+
+-- #check (inferInstance : RenMapEmpty Term)
+-- #check (inferInstance : RenMapVecDef Term Term [Ty])
+-- #check (inferInstance : RenMapId Term [Term, Ty])
+-- #check (inferInstance : RenMapCompose Term [Term, Ty])
+-- #check (inferInstance : RenMapVecDef Term Term [])
+-- #check (inferInstance : RenMapId Term [Term])
+-- #check (inferInstance : RenMapCompose Term [Term])
+-- #check (inferInstance : RenMapId Term [Ty])
+-- #check (inferInstance : RenMapCompose Term [Ty])
+
+-- -- smap
+-- #print Term.smap
+-- #print Term.smap._f
+
+-- #check (inferInstance : SubstMap Term [Term, Ty])
+-- #check (inferInstance : SubstSuffix Term [Ty])
+-- #check (inferInstance : SubstMap Term [Ty])
+-- #check (inferInstance : SubstMap Term [Term])
+-- #check (inferInstance : SubstSuffix Term [])
+-- #check (inferInstance : SubstMap Term [])
+-- #check (inferInstance : SubstMapAll [Term])
+-- #check (inferInstance : SubstMapAll [Term, Ty])
+
+-- #print Term.smap_empty -- remove
+-- #print Term.smap_fix
+
+-- #print Term.smap_term_var
+-- #print Term.smap_term_app
+-- #print Term.smap_term_lam
+-- #print Term.smap_term_tapp
+-- #print Term.smap_term_tlam
+-- #print Term.smap_term_zero
+-- #print Term.smap_term_succ
+-- #print Term.smap_term_nrec
+
+-- #print Term.smap_ty_var
+-- #print Term.smap_ty_app
+-- #print Term.smap_ty_lam
+-- #print Term.smap_ty_tapp
+-- #print Term.smap_ty_tlam
+-- #print Term.smap_ty_zero
+-- #print Term.smap_ty_succ
+-- #print Term.smap_ty_nrec
+
+-- #print Term.smap_term_ty_var
+-- #print Term.smap_term_ty_app
+-- #print Term.smap_term_ty_lam
+-- #print Term.smap_term_ty_tapp
+-- #print Term.smap_term_ty_tlam
+-- #print Term.smap_term_ty_zero
+-- #print Term.smap_term_ty_succ
+-- #print Term.smap_term_ty_nrec
+
+-- #print Term.from_action_smap
+-- #print Term.from_action_smap0
+-- #print Term.from_action_smap1
+
+-- #check (inferInstance : SuffixCommuteRenRen Term [Ty])
+-- #check (inferInstance : SuffixCommuteRenSub Term [Ty])
+-- #check (inferInstance : SuffixCommuteSubRen Term [Ty])
+-- #check (inferInstance : SubstMapEmpty Term)
+
+-- #check (inferInstance : SubstMapVecDef Term Term [Ty])
+-- #check (inferInstance : SubstMapId Term [Term, Ty])
+-- #check (inferInstance : SubstMapStable Term [Term, Ty])
+-- #check (inferInstance : SubstMapRenComposeLeft Term [Term, Ty])
+-- #check (inferInstance : SubstMapRenComposeRight Term [Term, Ty])
+
+-- #check (inferInstance : SubstMapVecDef Term Term [])
+-- #check (inferInstance : SubstMapId Term [Term])
+-- #check (inferInstance : SubstMapStable Term [Term])
+-- #check (inferInstance : SubstMapRenComposeLeft Term [Term])
+-- #check (inferInstance : SubstMapRenComposeRight Term [Term])
+
+-- #check (inferInstance : SubstMapId Term [Ty])
+-- #check (inferInstance : SubstMapStable Term [Ty])
+-- #check (inferInstance : SubstMapRenComposeLeft Term [Ty])
+-- #check (inferInstance : SubstMapRenComposeRight Term [Ty])
+
+-- #check (inferInstance : SubstMapCompose Term [Term, Ty])
+-- #check (inferInstance : SubstMapCompose Term [Ty])
+-- #check (inferInstance : SubstMapCompose Term [Term])
+
+----------------------------------------------------------------------------------------------------
+-- Ty Renaming & Substitution
+----------------------------------------------------------------------------------------------------
+@[coe]
+def Ty.from_action : Action Ty -> Ty
+| re y => var y
+| su t => t
+
+@[simp]
+theorem Ty.from_action_id {n} : from_action (𝐬0.act n) = var n := by
+  simp [from_action]
+
+@[simp]
+theorem Ty.from_action_succ {n} : from_action (𝐬1.act n) = var (n + 1) := by
+  simp [from_action]
+
+@[simp]
+theorem Ty.from_action_re {n} : from_action (re n) = var n := by simp [from_action]
+
+@[simp]
+theorem Ty.from_action_su {t} : from_action (su t) = t := by simp [from_action]
+
+instance : Coe (Action Ty) Ty where
+  coe := Ty.from_action
+
+@[simp]
+def Ty.rmap (r : RenVec [Ty]) : Ty -> Ty
+| var x => var (r.1.act x)
+| nat => nat
+| arrow t1 t2 => arrow (t1.rmap r) (t2.rmap r)
+| all t => all $ t.rmap $ r.lift [1]
+
+instance : RenMap Ty [Ty] where
+  rmap := Ty.rmap
+
+@[simp]
+theorem Ty.rmap_fix {r : RenVec [Ty]} {t : Ty} : rmap r t = t⟨r,⟩ := by simp [RenMap.rmap]
+
+instance : RenSuffix Ty [] := ⟨⟩
+instance : RenMap Ty [] where
+  rmap _ := id
+
+@[reducible, simp]
+instance instRenMapAll_Ty : RenMapAll [Ty] := .cons .nil
+
+@[simp]
+theorem Ty.rmap_var {x} {r : RenVec [Ty]} : (var x)⟨r,⟩ = .var (r.1.act x) := by
+  simp only [RenMap.rmap]; rw [rmap]
+
+@[simp]
+theorem Ty.rmap_nat {r : RenVec [Ty]} : (nat)⟨r,⟩ = nat := by
+  simp only [RenMap.rmap]; rw [rmap]
+
+@[simp]
+theorem Ty.rmap_arrow {t1 t2 : Ty} {r : RenVec [Ty]} : (arrow t1 t2)⟨r,⟩ = arrow t1⟨r,⟩ t2⟨r,⟩ := by
+  simp only [RenMap.rmap]; rw [rmap]
+
+@[simp]
+theorem Ty.rmap_all {t} {r : RenVec [Ty]} : (all t)⟨r,⟩ = all t⟨r.lift [1],⟩ := by
+  simp only [RenMap.rmap]; rw [rmap]
+
+@[simp]
+theorem Ty.from_action_rmap {t : Action Ty} {r : RenVec [Ty]}
+  : (from_action t)⟨r,⟩ = from_action t⟨r,⟩
+:= by cases t <;> simp
+
+instance : RenMapEmpty Ty where
+  apply_empty := by intro s; simp [RenMap.rmap]
+
+instance : RenMapId Ty [Ty] where
+  apply_id := by subst_solve_id
+
+instance : RenMapCompose Ty [Ty] where
+  apply_compose := by subst_solve_compose
+
+@[simp]
+def Ty.smap (σ : SubstVec [Ty]) : Ty -> Ty
+| var x => σ.1.act x
+| nat => nat
+| arrow t1 t2 => arrow (t1.smap σ) (t2.smap σ)
+| all t => all $ t.smap $ σ.lift [1]
+
+instance : SubstMap Ty [Ty] where
+  smap := Ty.smap
+
+@[simp]
+theorem Ty.smap_fix {σ : SubstVec [Ty]} {t : Ty} : smap σ t = t[σ,] := by simp [SubstMap.smap]
+
+instance : SubstSuffix Ty [] := ⟨⟩
+instance : SubstMap Ty [] where
+  smap _ := id
+
+@[reducible, simp]
+instance instSubstMapAll_Ty : SubstMapAll [Ty] := .cons .nil
+
+@[simp]
+theorem Ty.smap_var {x} {σ : SubstVec [Ty]} : (var x)[σ,] = σ.1.act x := by
+  simp only [SubstMap.smap]; rw [smap]
+
+@[simp]
+theorem Ty.smap_nat {σ : SubstVec [Ty]} : (nat)[σ,] = nat := by
+  simp only [SubstMap.smap]; rw [smap]
+
+@[simp]
+theorem Ty.smap_arrow {t1 t2 : Ty} {σ : SubstVec [Ty]} : (arrow t1 t2)[σ,] = arrow t1[σ,] t2[σ,] := by
+  simp only [SubstMap.smap]; rw [smap]
+
+@[simp]
+theorem Ty.smap_all {t} {σ : SubstVec [Ty]} : (all t)[σ,] = all t[σ.lift [1],] := by
+  simp only [SubstMap.smap]; rw [smap]
+
+@[simp]
+theorem Ty.from_action_smap {t : Action Ty} {σ : SubstVec [Ty]}
+  : (from_action t)[σ,] = from_action t[σ,]
+:= by cases t <;> simp
+
+instance : SubstMapEmpty Ty where
+  apply_empty := by intro s; simp [SubstMap.smap]
+
+instance : SubstMapId Ty [Ty] where
+  apply_id := by subst_solve_id
+
+instance : SubstMapStable Ty [Ty] where
+  apply_stable := by subst_solve_stable
+
+instance : SubstMapRenComposeLeft Ty [Ty] where
+  apply_ren_compose_left := by subst_solve_compose
+
+instance : SubstMapRenComposeRight Ty [Ty] where
+  apply_ren_compose_right := by subst_solve_compose
+
+instance : SubstMapCompose Ty [Ty] where
+  apply_compose := by subst_solve_compose
+
+----------------------------------------------------------------------------------------------------
+-- Term Renaming & Substitution
+----------------------------------------------------------------------------------------------------
+
+@[coe]
+def Term.from_action : Action Term -> Term
+| re y => var y
+| su t => t
+
+@[simp, grind =]
+theorem Term.from_action_id {n} : from_action (𝐬0.act n) = var n := by
+  simp [from_action]
+
+@[simp, grind =]
+theorem Term.from_action_succ {n} : from_action (𝐬1.act n) = var (n + 1) := by
+  simp [from_action]
+
+@[simp, grind =]
+theorem Term.from_acton_re {n} : from_action (re n) = var n := by simp [from_action]
+
+@[simp, grind =]
+theorem Term.from_action_su {t} : from_action (su t) = t := by simp [from_action]
+
+instance : Coe (Action Term) Term where
+  coe := Term.from_action
+
+@[simp]
+def Term.rmap (r : RenVec [Term, Ty]) : Term -> Term
+| var x => var (r.1.act x)
+| app t1 t2 => app (t1.rmap r) (t2.rmap r)
+| lam A t => lam A⟨r.2.1⟩ (t.rmap $ r.lift [1, 0])
+| tapp t A => tapp (t.rmap r) A⟨r.2.1⟩
+| tlam t => tlam (t.rmap $ r.lift [0, 1])
+| zero => zero
+| succ t => succ (t.rmap r)
+| nrec motive z s n => nrec motive⟨r.2.1⟩ (z.rmap r) (s.rmap $ r.lift [2, 1]) (n.rmap r)
+
+instance : RenMap Term [Term, Ty] where
+  rmap := Term.rmap
+
+@[simp]
+theorem Term.rmap_fix {r : RenVec [Term, Ty]} {t : Term} : rmap r t = t⟨r,⟩ := by simp [RenMap.rmap]
+
+@[simp]
+theorem Term.rmap_term_ty_var {x} {r : RenVec [Term, Ty]} : (var x)⟨r,⟩ = var (r.1.act x) := rfl
+
+@[simp]
+theorem Term.rmap_term_ty_app {t1 t2} {r : RenVec [Term, Ty]} : (app t1 t2)⟨r,⟩ = app t1⟨r,⟩ t2⟨r,⟩ := by
+  simp only [RenMap.rmap]; rw [rmap]
+
+@[simp]
+theorem Term.rmap_term_ty_lam'' {A t} {r : RenVec [Term, Ty]}
+  : (lam A t)⟨r,⟩ = lam A⟨r.2.1⟩ t⟨r.lift [1, 0],⟩
+:= by simp only [RenMap.rmap]; rw [rmap]; try simp
+
+@[simp]
+theorem Term.rmap_term_ty_tapp {t1 t2} {r : RenVec [Term, Ty]}
+  : (tapp t1 t2)⟨r,⟩ = tapp t1⟨r,⟩ t2⟨r.2.1⟩
+:= by simp only [RenMap.rmap]; rw [rmap]; try simp
+
+@[simp]
+theorem Term.rmap_term_ty_tlam {t} {r : RenVec [Term, Ty]} : (tlam t)⟨r,⟩ = tlam t⟨r.lift [0, 1],⟩ := by
+  simp only [RenMap.rmap]; rw [rmap]; try simp
+
+@[simp]
+theorem Term.rmap_term_ty_zero {r : RenVec [Term, Ty]} : zero⟨r,⟩ = zero := by
+  simp only [RenMap.rmap]; rw [rmap]; try simp
+
+@[simp]
+theorem Term.rmap_term_ty_succ {t} {r : RenVec [Term, Ty]} : (succ t)⟨r,⟩ = succ t⟨r,⟩ := by
+  simp only [RenMap.rmap]; rw [rmap]; try simp
+
+@[simp]
+theorem Term.rmap_term_ty_nrec {m z s n} {r : RenVec [Term, Ty]}
+  : (nrec m z s n)⟨r,⟩ = nrec m⟨r.2.1⟩ z⟨r,⟩ s⟨r.lift [2, 1],⟩ n⟨r,⟩
+:= by simp only [RenMap.rmap]; rw [rmap]; try simp
+
+instance : RenSuffix Term [Ty] := ⟨⟩
+instance : RenMap Term [Ty] where
+  rmap r := Term.rmap (Ren.id Term, r.1, .nil)
+
+@[simp]
+theorem Term.rmap_ty_var {x} {r : RenVec [Ty]} : (var x)⟨r,⟩ = var x := by
+  simp only [RenMap.rmap]; rw [rmap]; try simp
+
+@[simp]
+theorem Term.rmap_ty_app {t1 t2} {r : RenVec [Ty]} : (app t1 t2)⟨r,⟩ = app t1⟨r,⟩ t2⟨r,⟩ := by
+  simp only [RenMap.rmap]; rw [rmap]; try simp
+
+@[simp]
+theorem Term.rmap_ty_lam {A t} {r : RenVec [Ty]}
+  : (lam A t)⟨r,⟩ = lam A⟨r.1⟩ t⟨r,⟩
+:= by simp only [RenMap.rmap]; rw [rmap]; try simp
+
+@[simp]
+theorem Term.rmap_ty_tapp {t1 t2} {r : RenVec [Ty]}
+  : (tapp t1 t2)⟨r,⟩ = tapp t1⟨r,⟩ t2⟨r.1⟩
+:= by simp only [RenMap.rmap]; rw [rmap]; try simp
+
+@[simp]
+theorem Term.rmap_ty_tlam {t} {r : RenVec [Ty]} : (tlam t)⟨r,⟩ = tlam t⟨r.lift [1],⟩ := by
+  simp only [RenMap.rmap]; rw [rmap]; try simp
+
+@[simp]
+theorem Term.rmap_ty_zero {r : RenVec [Ty]} : zero⟨r,⟩ = zero := by
+  simp only [RenMap.rmap]; rw [rmap]; try simp
+
+@[simp]
+theorem Term.rmap_ty_succ {t} {r : RenVec [Ty]} : (succ t)⟨r,⟩ = succ t⟨r,⟩ := by
+  simp only [RenMap.rmap]; rw [rmap]; try simp
+
+@[simp]
+theorem Term.rmap_ty_nrec {m z s n} {r : RenVec [Ty]}
+  : (nrec m z s n)⟨r,⟩ = nrec m⟨r.1⟩ z⟨r,⟩ s⟨r.lift [1],⟩ n⟨r,⟩
+:= by simp only [RenMap.rmap]; rw [rmap]; try simp
+
+instance : RenMap Term [Term] where
+  rmap r := Term.rmap (r.1, Ren.id Ty, .nil)
+
+@[simp]
+theorem Term.rmap_term_var {x} {r : RenVec [Term]} : (var x)⟨r,⟩ = var (r.1.act x) := by
+  simp only [RenMap.rmap]; rw [rmap]; try simp
+
+@[simp]
+theorem Term.rmap_term_app {t1 t2} {r : RenVec [Term]} : (app t1 t2)⟨r,⟩ = app t1⟨r,⟩ t2⟨r,⟩ := by
+  simp only [RenMap.rmap]; rw [rmap]; try simp
+
+@[simp]
+theorem Term.rmap_term_lam' {A t} {r : RenVec [Term]}
+  : (lam A t)⟨r,⟩ = lam A t⟨r.lift [1],⟩
+:= by simp only [RenMap.rmap]; rw [rmap]; try simp
+
+@[simp]
+theorem Term.rmap_term_tapp {t1 t2} {r : RenVec [Term]}
+  : (tapp t1 t2)⟨r,⟩ = tapp t1⟨r,⟩ t2
+:= by simp only [RenMap.rmap]; rw [rmap]; try simp
+
+@[simp]
+theorem Term.rmap_term_tlam {t} {r : RenVec [Term]} : (tlam t)⟨r,⟩ = tlam t⟨r,⟩ := by
+  simp only [RenMap.rmap]; rw [rmap]; try simp
+
+@[simp]
+theorem Term.rmap_term_zero {r : RenVec [Term]} : zero⟨r,⟩ = zero := by
+  simp only [RenMap.rmap]; rw [rmap]; try simp
+
+@[simp]
+theorem Term.rmap_term_succ {t} {r : RenVec [Term]} : (succ t)⟨r,⟩ = succ t⟨r,⟩ := by
+  simp only [RenMap.rmap]; rw [rmap]; try simp
+
+@[simp]
+theorem Term.rmap_term_nrec {m z s n} {r : RenVec [Term]}
+  : (nrec m z s n)⟨r,⟩ = nrec m z⟨r,⟩ s⟨r.lift [2],⟩ n⟨r,⟩
+:= by simp only [RenMap.rmap]; rw [rmap]; try simp
+
+@[simp]
+theorem Term.from_action_rmap {t : Action Term} {r : RenVec [Term, Ty]}
+  : (from_action t)⟨r,⟩ = from_action t⟨r,⟩
+:= by cases t <;> simp [from_action]
+
+@[simp]
+theorem Term.from_action_rmap0 {t : Action Term} {r : RenVec [Term]}
+  : (from_action t)⟨r,⟩ = from_action t⟨r,⟩
+:= by cases t <;> simp [from_action]
+
+@[simp]
+theorem Term.from_action_rmap1 {t : Action Term} {r : RenVec [Ty]}
+  : (from_action t)⟨r,⟩ = from_action t⟨r,⟩
+:= by cases t <;> simp [from_action]
+
+instance : RenSuffix Term [] := ⟨⟩
+instance : RenMap Term [] where
+  rmap _ := id
+
+@[reducible, simp]
+instance instRenMapAll_Term : RenMapAll [Term] := .cons .nil
+
+@[reducible, simp]
+instance instRenMapAll_Term_Ty : RenMapAll [Term, Ty] := .cons instRenMapAll_Ty
+
+instance : RenMapEmpty Term where
+  apply_empty := by intro s; simp [RenMap.rmap]
+
+instance : RenMapVecDef Term Term [Ty] where
+  apply_vecdef := by intro s r; induction s generalizing r <;> simp [*]
+
+instance : RenMapId Term [Term, Ty] where
+  apply_id := by subst_solve_id
+
+instance : RenMapCompose Term [Term, Ty] where
+  apply_compose := by subst_solve_compose
+
+instance : RenMapVecDef Term Term [] where
+  apply_vecdef := by intro s r; induction s generalizing r <;> simp [*]
+
+instance : RenMapId Term [Term] where
+  apply_id := by subst_solve_id
+
+instance : RenMapCompose Term [Term] where
+  apply_compose := by subst_solve_compose
+
+instance : RenMapId Term [Ty] where
+  apply_id := by subst_solve_id
+
+instance : RenMapCompose Term [Ty] where
+  apply_compose := by subst_solve_compose
+
+@[simp]
+def Term.smap (σ : SubstVec [Term, Ty]) : Term -> Term
+| var x => σ.1.act x
+| app t1 t2 => app (t1.smap σ) (t2.smap σ)
+| lam A t => lam A[σ.2.1] (t.smap $ σ.lift [1, 0])
+| tapp t A => tapp (t.smap σ) A[σ.2.1]
+| tlam t => tlam (t.smap $ σ |> .lift [0, 1] |> .ren Term [Ty] (𝐫1, .nil) 0 rfl)
+| zero => zero
+| succ t => succ (t.smap σ)
+| nrec motive z s n =>
+  nrec motive[σ.2.1] (z.smap σ) (s.smap $ σ |> .lift [2, 1] |> .ren Term [Ty] (𝐫1, .nil) 0 rfl) (n.smap σ)
+
+instance : SubstMap Term [Term, Ty] where
+  smap := Term.smap
+
+@[simp]
+theorem Term.smap_fix {σ : SubstVec [Term, Ty]} {t : Term} : smap σ t = t[σ,] := by
+  simp [SubstMap.smap]
+
+@[simp]
+theorem Term.smap_term_ty_var {x} {σ : SubstVec [Term, Ty]} : (var x)[σ,] = σ.1.act x := by
+  simp only [SubstMap.smap]; rw [smap]; try simp
+
+@[simp]
+theorem Term.smap_term_ty_app {t1 t2} {σ : SubstVec [Term, Ty]} : (app t1 t2)[σ,] = app t1[σ,] t2[σ,] := by
+  simp only [SubstMap.smap]; rw [smap]; try simp
+
+@[simp]
+theorem Term.smap_term_ty_lam {A t} {σ : SubstVec [Term, Ty]}
+  : (lam A t)[σ,] = lam A[σ.2.1] t[σ.lift [1, 0],]
+:= by simp only [SubstMap.smap]; rw [smap]; try simp
+
+@[simp]
+theorem Term.smap_term_ty_tapp {t1 t2} {σ : SubstVec [Term, Ty]}
+  : (tapp t1 t2)[σ,] = tapp t1[σ,] t2[σ.2.1]
+:= by simp only [SubstMap.smap]; rw [smap]; try simp
+
+@[simp]
+theorem Term.smap_term_ty_tlam {t} {σ : SubstVec [Term, Ty]}
+  : (tlam t)[σ,] = tlam t[σ |> .lift [0, 1] |> .ren Term [Ty] (𝐫1, .nil) 0 rfl,]
+:= by simp only [SubstMap.smap]; rw [smap]; try simp
+
+@[simp]
+theorem Term.smap_term_ty_zero {σ : SubstVec [Term, Ty]} : zero[σ,] = zero := by
+  simp only [SubstMap.smap]; rw [smap]; try simp
+
+@[simp]
+theorem Term.smap_term_ty_succ {t} {σ : SubstVec [Term, Ty]} : (succ t)[σ,] = succ t[σ,] := by
+  simp only [SubstMap.smap]; rw [smap]; try simp
+
+@[simp]
+theorem Term.smap_term_ty_nrec {m z s n} {σ : SubstVec [Term, Ty]}
+  : (nrec m z s n)[σ,] = nrec m[σ.2.1] z[σ,] s[σ |> .lift [2, 1] |> .ren Term [Ty] (𝐫1, .nil) 0 rfl,] n[σ,]
+:= by simp only [SubstMap.smap]; rw [smap]; try simp
+
+@[simp]
+theorem Term.from_action_smap {t : Action Term} {σ : SubstVec [Term, Ty]}
+  : (from_action t)[σ,] = from_action t[σ,]
+:= by cases t <;> simp [from_action]
+
+instance : SubstSuffix Term [Ty] := ⟨⟩
+@[simp]
+instance : SubstMap Term [Ty] where
+  smap σ := Term.smap (Subst.id Term, σ.1, .nil)
+
+@[simp]
+theorem Term.smap_ty_var {x} {σ : SubstVec [Ty]} : (var x)[σ,] = var x := by
+  simp only [SubstMap.smap]; rw [smap]; try simp
+
+@[simp]
+theorem Term.smap_ty_app {t1 t2} {σ : SubstVec [Ty]} : (app t1 t2)[σ,] = app t1[σ,] t2[σ,] := by
+  simp only [SubstMap.smap]; rw [smap]; try simp
+
+@[simp]
+theorem Term.smap_ty_lam {A t} {σ : SubstVec [Ty]}
+  : (lam A t)[σ,] = lam A[σ.1] t[σ,]
+:= by simp only [SubstMap.smap]; rw [smap]; try simp
+
+@[simp]
+theorem Term.smap_ty_tapp {t1 t2} {σ : SubstVec [Ty]}
+  : (tapp t1 t2)[σ,] = tapp t1[σ,] t2[σ.1]
+:= by simp only [SubstMap.smap]; rw [smap]; try simp
+
+@[simp]
+theorem Term.smap_ty_tlam {t} {σ : SubstVec [Ty]}
+  : (tlam t)[σ,] = tlam t[σ |> .lift [1],]
+:= by simp only [SubstMap.smap]; rw [smap]; try simp
+
+@[simp]
+theorem Term.smap_ty_zero {σ : SubstVec [Ty]} : zero[σ,] = zero := by
+  simp only [SubstMap.smap]; rw [smap]; try simp
+
+@[simp]
+theorem Term.smap_ty_succ {t} {σ : SubstVec [Ty]} : (succ t)[σ,] = succ t[σ,] := by
+  simp only [SubstMap.smap]; rw [smap]; try simp
+
+@[simp]
+theorem Term.smap_ty_nrec {m z s n} {σ : SubstVec [Ty]}
+  : (nrec m z s n)[σ,] = nrec m[σ.1] z[σ,] s[σ |> .lift [1],] n[σ,]
+:= by simp only [SubstMap.smap]; rw [smap]; try simp
+
+@[simp]
+theorem Term.from_action_smap1 {t : Action Term} {σ : SubstVec [Ty]}
+  : (from_action t)[σ,] = from_action t[σ,]
+:= by cases t <;> simp [from_action]
+
+@[simp]
+instance : SubstMap Term [Term] where
+  smap σ := Term.smap (σ.1, Subst.id Ty, .nil)
+
+@[simp]
+theorem Term.smap_term_var {x} {σ : SubstVec [Term]} : (var x)[σ,] = σ.1.act x := by
+  simp only [SubstMap.smap]; rw [smap]; try simp
+
+@[simp]
+theorem Term.smap_term_app {t1 t2} {σ : SubstVec [Term]} : (app t1 t2)[σ,] = app t1[σ,] t2[σ,] := by
+  simp only [SubstMap.smap]; rw [smap]; try simp
+
+@[simp]
+theorem Term.smap_term_lam {A t} {σ : SubstVec [Term]}
+  : (lam A t)[σ,] = lam A t[σ.lift [1],]
+:= by simp only [SubstMap.smap]; rw [smap]; try simp
+
+@[simp]
+theorem Term.smap_term_tapp {t1 t2} {σ : SubstVec [Term]}
+  : (tapp t1 t2)[σ,] = tapp t1[σ,] t2
+:= by simp only [SubstMap.smap]; rw [smap]; try simp
+
+@[simp]
+theorem Term.smap_term_tlam {t} {σ : SubstVec [Term]}
+  : (tlam t)[σ,] = tlam t[σ |> .ren Term [Ty] (𝐫1, .nil) 0 rfl,]
+:= by simp only [SubstMap.smap]; rw [smap]; try simp
+
+@[simp]
+theorem Term.smap_term_zero {σ : SubstVec [Term]} : zero[σ,] = zero := by
+  simp only [SubstMap.smap]; rw [smap]; try simp
+
+@[simp]
+theorem Term.smap_term_succ {t} {σ : SubstVec [Term]} : (succ t)[σ,] = succ t[σ,] := by
+  simp only [SubstMap.smap]; rw [smap]; try simp
+
+@[simp]
+theorem Term.smap_term_nrec {m z s n} {σ : SubstVec [Term]}
+  : (nrec m z s n)[σ,] = nrec m z[σ,] s[σ |> .lift [2] |> .ren Term [Ty] (𝐫1, .nil) 0 rfl,] n[σ,]
+:= by simp only [SubstMap.smap]; rw [smap]; try simp
+
+@[simp]
+theorem Term.from_action_smap0 {t : Action Term} {σ : SubstVec [Term]}
+  : (from_action t)[σ,] = from_action t[σ,]
+:= by cases t <;> simp [from_action]
+
+instance : SubstSuffix Term [] := ⟨⟩
+instance : SubstMap Term [] where
+  smap _ := id
+
+@[reducible, simp]
+instance instSubstMapAll_Term : SubstMapAll [Term] := .cons .nil
+
+@[reducible, simp]
+instance instSubstMapAll_Term_Ty : SubstMapAll [Term, Ty] := .cons instSubstMapAll_Ty
+
+instance : SubstMapEmpty Term where
+  apply_empty := by intro s; simp [SubstMap.smap]
+
+instance : SubstMapVecDef Term Term [] where
+  apply_vecdef := by intro s σ; induction s generalizing σ <;> simp [*]
+
+-- The `[Ty]` Suffix:
+instance : SuffixCommuteRenRen Term [Ty] where
+  ren_ren := by subst_solve_compose
+
+instance : SuffixCommuteRenSub Term [Ty] where
+  ren_sub := by subst_solve_compose
+
+instance : SuffixCommuteSubRen Term [Ty] where
+  sub_ren := by subst_solve_compose
+
+instance : SubstMapVecDef Term Term [Ty] where
+  apply_vecdef := by intro s σ; induction s generalizing σ <;> simp [*]
+
+instance : SubstMapId Term [Ty] where
+  apply_id := by subst_solve_id
+
+instance : SubstMapStable Term [Ty] where
+  apply_stable := by sorry --subst_solve_stable
+
+instance : SubstMapRenComposeLeft Term [Ty] where
+  apply_ren_compose_left := by subst_solve_compose
+
+instance : SubstMapRenComposeRight Term [Ty] where
+  apply_ren_compose_right := by subst_solve_compose
+
+instance : SubstMapCompose Term [Ty] where
+  apply_compose := by subst_solve_compose
+
+-- The `[Term]` Singleton:
+instance : SubstMapId Term [Term] where
+  apply_id := by subst_solve_id
+
+instance : SubstMapStable Term [Term] where
+  apply_stable := by sorry --subst_solve_stable
+
+instance : SubstMapRenComposeLeft Term [Term] where
+  apply_ren_compose_left := by subst_solve_compose
+
+instance : SubstMapRenComposeRight Term [Term] where
+  apply_ren_compose_right := by subst_solve_compose
+
+instance : SubstMapCompose Term [Term] where
+  apply_compose := by subst_solve_compose
+
+-- The `[Term, Ty]` Original:
+instance : SubstMapId Term [Term, Ty] where
+  apply_id := by subst_solve_id
+
+instance : SubstMapStable Term [Term, Ty] where
+  apply_stable := by sorry --subst_solve_stable
+
+instance : SubstMapRenComposeLeft Term [Term, Ty] where
+  apply_ren_compose_left := by subst_solve_compose
+
+instance : SubstMapRenComposeRight Term [Term, Ty] where
+  apply_ren_compose_right := by subst_solve_compose
+
+instance : SubstMapCompose Term [Term, Ty] where
+  apply_compose := by subst_solve_compose
 
 end SystemFWithNat
