LeanSubst/Rewriting/Normal.lean
@@ -3,121 +3,121 @@ import Init.WF
 import LeanSubst.Laws
 import LeanSubst.Rewriting.Reduction
 
--- namespace LeanSubst
---   universe u
+namespace LeanSubst
+  universe u
 
---   section
---     variable {T : Type}
+  section
+    variable {T : Type}
 
---     def Reducible (R : T -> T -> Prop) (t : T) := ∃ t', R t t'
---     def Normal (R : T -> T -> Prop) (t : T) := ¬ (Reducible R t)
---     def NormalForm (R : T -> T -> Prop) (t : T) (t' : T) := Star R t t' ∧ Normal R t'
---     def WN (R : T -> T -> Prop) (t : T) := ∃ t', NormalForm R t t'
+    def Reducible (R : T -> T -> Prop) (t : T) := ∃ t', R t t'
+    def Normal (R : T -> T -> Prop) (t : T) := ¬ (Reducible R t)
+    def NormalForm (R : T -> T -> Prop) (t : T) (t' : T) := Star R t t' ∧ Normal R t'
+    def WN (R : T -> T -> Prop) (t : T) := ∃ t', NormalForm R t t'
 
---     inductive SN (R : T -> T -> Prop) : T -> Prop where
---     | sn {x} : (∀ y, R x y -> SN R y) -> SN R x
+    inductive SN (R : T -> T -> Prop) : T -> Prop where
+    | sn {x} : (∀ y, R x y -> SN R y) -> SN R x
 
---     inductive SNPlus (R : T -> T -> Prop) : T -> Prop where
---     | sn {x} : (∀ y, Plus R x y -> SNPlus R y) -> SNPlus R x
+    inductive SNPlus (R : T -> T -> Prop) : T -> Prop where
+    | sn {x} : (∀ y, Plus R x y -> SNPlus R y) -> SNPlus R x
 
---     variable {R R1 R2 : T -> T -> Prop}
+    variable {R R1 R2 : T -> T -> Prop}
 
---     namespace SNPlus
---       theorem impies_sn {t} : SNPlus R t -> SN R t := by
---         intro h; induction h; case _ t' _ ih =>
---         constructor; intro t'' r
---         apply ih t'' (Plus.start r)
+    namespace SNPlus
+      theorem impies_sn {t} : SNPlus R t -> SN R t := by
+        intro h; induction h; case _ t' _ ih =>
+        constructor; intro t'' r
+        apply ih t'' (Plus.start r)
 
---       theorem preservation_step {t t'} : SNPlus R t -> R t t' -> SNPlus R t' := by
---         intro h r; induction h; case _ z h _ =>
---           apply h _ (Plus.start r)
+      theorem preservation_step {t t'} : SNPlus R t -> R t t' -> SNPlus R t' := by
+        intro h r; induction h; case _ z h _ =>
+          apply h _ (Plus.start r)
 
---       theorem preservation {t t'} : SNPlus R t -> Star R t t' -> SNPlus R t' := by
---         intro h r; induction r
---         case _ => apply h
---         case _ _ r2 ih =>
---           apply preservation_step ih r2
---     end SNPlus
+      theorem preservation {t t'} : SNPlus R t -> Star R t t' -> SNPlus R t' := by
+        intro h r; induction r
+        case _ => apply h
+        case _ _ r2 ih =>
+          apply preservation_step ih r2
+    end SNPlus
 
---     namespace SN
---       theorem preimage (f : T -> T) x :
---         (∀ x y, R x y -> R (f x) (f y)) ->
---         SN R (f x) ->
---         SN R x
---       := by
---         intro h sh
---         generalize zdef : f x = z at sh
---         induction sh generalizing f x
---         case _ x' h' ih =>
---           subst zdef; constructor
---           intro y r
---           apply ih (f y) (h _ _ r) f y h rfl
+    namespace SN
+      theorem preimage (f : T -> T) x :
+        (∀ x y, R x y -> R (f x) (f y)) ->
+        SN R (f x) ->
+        SN R x
+      := by
+        intro h sh
+        generalize zdef : f x = z at sh
+        induction sh generalizing f x
+        case _ x' h' ih =>
+          subst zdef; constructor
+          intro y r
+          apply ih (f y) (h _ _ r) f y h rfl
 
---       theorem preservation_step {t t'} : SN R t -> R t t' -> SN R t' := by
---         intro h red
---         induction h
---         case _ z h1 _h2 =>
---           apply h1 _ red
+      theorem preservation_step {t t'} : SN R t -> R t t' -> SN R t' := by
+        intro h red
+        induction h
+        case _ z h1 _h2 =>
+          apply h1 _ red
 
---       theorem preservation {t t'} : SN R t -> Star R t t' -> SN R t' := by
---         intro h red
---         induction red
---         case _ => simp [*]
---         case _ _ r2 ih => apply preservation_step ih r2
+      theorem preservation {t t'} : SN R t -> Star R t t' -> SN R t' := by
+        intro h red
+        induction red
+        case _ => simp [*]
+        case _ _ r2 ih => apply preservation_step ih r2
 
---       theorem star {t} : (∀ y, Star R t y -> SN R y) -> SN R t := by
---         intro h
---         constructor
---         intro y r
---         apply h y (Star.step Star.refl r)
+      theorem star {t} : (∀ y, Star R t y -> SN R y) -> SN R t := by
+        intro h
+        constructor
+        intro y r
+        apply h y (Star.step Star.refl r)
 
---       theorem implies_snplus {t} : SN R t -> SNPlus R t := by
---         intro h; induction h; case _ t' _ ih =>
---         constructor; intro t'' r
---         have lem := Plus.destruct r
---         cases lem; case _ z lem =>
---           have lem2 := ih z lem.1
---           apply SNPlus.preservation lem2 lem.2
+      theorem implies_snplus {t} : SN R t -> SNPlus R t := by
+        intro h; induction h; case _ t' _ ih =>
+        constructor; intro t'' r
+        have lem := Plus.destruct r
+        cases lem; case _ z lem =>
+          have lem2 := ih z lem.1
+          apply SNPlus.preservation lem2 lem.2
 
---       theorem expansion_step {t t' : T} (f : FunctionalTerm R t) : SN R t' -> R t t' -> SN R t := by
---         intro h r
---         apply SN.sn; intro y r'
---         rw [<-f r r']
---         apply h
+      theorem expansion_step {t t' : T} (f : FunctionalTerm R t) : SN R t' -> R t t' -> SN R t := by
+        intro h r
+        apply SN.sn; intro y r'
+        rw [<-f r r']
+        apply h
 
---       theorem expansion {t t' : T} [Functional R] : SN R t' -> Star R t t' -> SN R t := by
---         intro h r
---         induction r; apply h
---         case _ r1 r2 ih =>
---           have lem := expansion_step Functional.functional h r2
---           apply ih lem
+      theorem expansion {t t' : T} [Functional R] : SN R t' -> Star R t t' -> SN R t := by
+        intro h r
+        induction r; apply h
+        case _ r1 r2 ih =>
+          have lem := expansion_step Functional.functional h r2
+          apply ih lem
 
---       theorem equiv_acc {t} : SN R t <-> Acc (flip $ R) t := by
---         apply Iff.intro
---         case _ =>
---           intro h; induction h
---           case _ x h ih =>
---           constructor
---           simp [flip]
---           exact ih
---         case _ =>
---           intro h; induction h
---           case _ x h ih =>
---           constructor
---           simp [flip] at ih
---           exact ih
+      theorem equiv_acc {t} : SN R t <-> Acc (flip $ R) t := by
+        apply Iff.intro
+        case _ =>
+          intro h; induction h
+          case _ x h ih =>
+          constructor
+          simp [flip]
+          exact ih
+        case _ =>
+          intro h; induction h
+          case _ x h ih =>
+          constructor
+          simp [flip] at ih
+          exact ih
 
---       theorem wellfounded : (∀ t, SN R t) -> WellFounded (flip $ R) := by
---         intro h; constructor
---         intro a; replace h := h a
---         apply equiv_acc.1 h
+      theorem wellfounded : (∀ t, SN R t) -> WellFounded (flip $ R) := by
+        intro h; constructor
+        intro a; replace h := h a
+        apply equiv_acc.1 h
 
---       variable [RenMap T T] [SubstMap T T] [Substitutive R]
+      -- variable [RenMap T T] [SubstMap T T] [Substitutive R]
 
---       theorem subst_preimage {σ : Subst T} {t} : SN R t[σ] -> SN R t := by
---         intro r; apply preimage (smap σ) t _ r
---         intro x y r; apply Substitutive.subst
---         apply r
---     end SN
---   end
--- end LeanSubst
+      -- theorem subst_preimage {σ : Subst T} {t} : SN R t[σ] -> SN R t := by
+      --   intro r; apply preimage (smap σ) t _ r
+      --   intro x y r; apply Substitutive.subst
+      --   apply r
+    end SN
+  end
+end LeanSubst
