Examples.lean
@@ -1,8 +1,10 @@
 
-import Examples.CCOmegaVarSorted
 import Examples.STLC
-import Examples.SystemFWithNat
 import Examples.VariadicSTLC
+import Examples.SystemFWithNat
+import Examples.SystemFCallByValue
+import Examples.Symbolic
+import Examples.CCOmegaVarSorted
 
 def main : IO Unit :=
   IO.println s!"Examples Build"
