Examples/STLC.lean
@@ -1,2 +1,4 @@
 
 import Examples.STLC.Term
+import Examples.STLC.Theory
+import Examples.STLC.Normalization
